Verification mismatch fixed, extension and CLI both verify.

src/pathfind.dfy
@@ -11,57 +11,74 @@ module Pathfind {
   export
     provides Utils
     reveals Pathfinder
-    provides Pathfinder.grid
-    provides Pathfinder.rectangles
-    provides Pathfinder.Pathfind
+    provides Pathfinder.grid, Pathfinder.Valid, Pathfinder.Pathfind
 
   class Pathfinder<T> {
     const grid: array2<T>
-    const rectangles: array<UtilsPrivate.Rectangle>
+    const rectangles: seq<UtilsPrivate.Rectangle>
     const visibility_blocking: T -> bool
     const traversable: T -> bool
 
+    ghost predicate Valid()
+      reads this, grid
+    {
+      forall j :: 0 <= j < |rectangles| ==>
+                    UtilsPrivate.RectangleInRange(rectangles[j], grid)
+    }
+
     constructor(grid: array2<T>, visibility_blocking: T -> bool, traversable: T -> bool)
       ensures this.grid == grid
-      ensures forall j :: 0 <= j < rectangles.Length ==>
-                            UtilsPrivate.RectangleInRange(rectangles[j], grid)
+      ensures Valid()
     {
-      var rectangles_seq := ExtractBlockingRectangles(grid, visibility_blocking);
+      var rectangles0 := ExtractBlockingRectangles(grid, visibility_blocking);
       this.grid := grid;
-      this.rectangles := rectangles_seq;
+      this.rectangles := rectangles0;
       this.visibility_blocking := visibility_blocking;
       this.traversable := traversable;
     }
 
-    method Pathfind(agent_position: Utils.Point, value: (Utils.Point, Utils.Point, T) -> real) returns (path: seq<Utils.Point>, visible: array2<bool>)
+    method Pathfind(
+      agent_position: Utils.Point,
+      value: (Utils.Point, Utils.Point, T) -> real)
+      returns (path: seq<Utils.Point>, visible: array2<bool>)
+      requires Valid()
       requires Utils.ValidPoint(agent_position, grid)
-      requires  forall j :: 0 <= j < rectangles.Length ==>
-                              UtilsPrivate.RectangleInRange(rectangles[j], grid)
+      ensures Valid()
       ensures grid.Length0 == visible.Length0 && grid.Length1 == visible.Length1
       ensures forall p :: p in path ==> Utils.ValidPoint(p, grid)
-      // Should the ensures from FOV and A_Star be carried over here?
     {
+      var rectangles_array := new UtilsPrivate.Rectangle[|rectangles|](
+                                                         i requires 0 <= i < |rectangles| => rectangles[i]);
+      assert forall j :: 0 <= j < rectangles_array.Length ==> UtilsPrivate.RectangleInRange(rectangles_array[j], grid) by {
+        forall j | 0 <= j < rectangles_array.Length
+          ensures UtilsPrivate.RectangleInRange(rectangles_array[j], grid)
+        {
+          assert rectangles_array[j] == rectangles[j];
+        }
+      }
       var extended_rectangles := [];
-      visible, extended_rectangles := CalculateFOV(grid, rectangles, agent_position);
-      var goal := GetGoal(grid, visible, value, agent_position);
+      visible, extended_rectangles := CalculateFOV(grid, rectangles_array, agent_position);
+      var goal := GetGoal(visible, value, agent_position);
       path := A_Star(grid, agent_position, goal, traversable);
     }
 
-    // Call once during initialization to extract rectangles from the grid then use those rectangles for all future FOV calls.
-    static method ExtractBlockingRectangles(grid: array2<T>, visibility_blocking: T -> bool) returns (rectangles: array<UtilsPrivate.Rectangle>)
-      ensures forall i :: 0 <= i < rectangles.Length ==> UtilsPrivate.RectangleInRange(rectangles[i], grid)
-      ensures forall i :: 0 <= i < rectangles.Length ==> UtilsPrivate.RectangleMatchesGrid(rectangles[i], grid, visibility_blocking)
+    // Call once during initialization to extract rectangles from the grid,
+    // then reuse that cached sequence for future FOV calls.
+    static method ExtractBlockingRectangles(grid: array2<T>, visibility_blocking: T -> bool)
+      returns (rectangles: seq<UtilsPrivate.Rectangle>)
+      ensures forall i :: 0 <= i < |rectangles| ==> UtilsPrivate.RectangleInRange(rectangles[i], grid)
+      ensures forall i :: 0 <= i < |rectangles| ==> UtilsPrivate.RectangleMatchesGrid(rectangles[i], grid, visibility_blocking)
     {
-      var rectangles_seq := [];
+      rectangles := [];
       var visited := new bool[grid.Length0, grid.Length1]((i, j) => false);
 
       for x := 0 to grid.Length0
-        invariant forall r :: r in rectangles_seq ==> UtilsPrivate.RectangleInRange(r, grid)
-        invariant forall r :: r in rectangles_seq ==> UtilsPrivate.RectangleMatchesGrid(r, grid, visibility_blocking)
+        invariant forall r :: r in rectangles ==> UtilsPrivate.RectangleInRange(r, grid)
+        invariant forall r :: r in rectangles ==> UtilsPrivate.RectangleMatchesGrid(r, grid, visibility_blocking)
       {
         for y := 0 to grid.Length1
-          invariant forall r :: r in rectangles_seq ==> UtilsPrivate.RectangleInRange(r, grid)
-          invariant forall r :: r in rectangles_seq ==> UtilsPrivate.RectangleMatchesGrid(r, grid, visibility_blocking)
+          invariant forall r :: r in rectangles ==> UtilsPrivate.RectangleInRange(r, grid)
+          invariant forall r :: r in rectangles ==> UtilsPrivate.RectangleMatchesGrid(r, grid, visibility_blocking)
         {
           if visibility_blocking(grid[x, y]) && !visited[x, y] {
 
@@ -85,30 +102,29 @@ module Pathfind {
               y_size := y_size + 1;
             }
 
-            // Mark visited
+            // Mark visited.
             for xx := x to x + x_size {
               for yy := y to y + y_size {
                 visited[xx, yy] := true;
               }
             }
 
-            rectangles_seq := rectangles_seq + [UtilsPrivate.Rectangle(x, y, x + x_size, y + y_size)];
+            rectangles := rectangles + [UtilsPrivate.Rectangle(x, y, x + x_size, y + y_size)];
           }
         }
       }
-
-      rectangles := new UtilsPrivate.Rectangle[|rectangles_seq|](i requires 0 <= i < |rectangles_seq| => rectangles_seq[i]);
     }
 
-    method GetGoal<T>(grid: array2<T>, visible: array2<bool>, value_function: ((Utils.Point, Utils.Point, T) -> real), agent_position: Utils.Point)
+    method GetGoal(
+      visible: array2<bool>,
+      value_function: (Utils.Point, Utils.Point, T) -> real,
+      agent_position: Utils.Point)
       returns (goal: Utils.Point)
       requires grid.Length0 == visible.Length0 && grid.Length1 == visible.Length1
     {
-      goal := agent_position; // Default to current position if no visible cells have value > 0.
+      goal := agent_position; // Default to current position if no visible cell has value > 0.
 
-      // Find the best value among visible cells.
       var best_value := 0.0;
-      var distance := 0;
 
       for x := 0 to grid.Length0 {
         for y := 0 to grid.Length1 {
